Invariance Thesis for L w.r.t. Termination, Direction TM to L

theories/L/Functions/UnboundIteration.v
@@ -9,26 +9,27 @@ Section uiter.
   Variable f : X -> X + Y.
 
   Variable fT : timeComplexity (X -> X + Y).
-  Context `{computableTime' f fT}.
 
   Import HOAS_Notations.
-  Definition uiter := Eval cbn -[enc] in rho [L_HOAS (λ uiter x, !!(extT f) x (λ x' _ , uiter x') (λ y _ , y) !!I)].
+  Definition uiter := Eval cbn -[enc] in rho [L_HOAS (λ uiter f x, f x (λ x' _ , uiter f x') (λ y _ , y) !!I)].
   
   Lemma uiter_proc : proc uiter.
   Proof. unfold uiter. Lproc. Qed.
   Hint Resolve uiter_proc : LProc.
 
+  Context `{computableTime' f fT}.
+
   Fixpoint uiterTime n x :=
     match n with
       0 => 0
-    | S n' => fst (fT x tt) + 9 + match f x with
+    | S n' => fst (fT x tt) + 11 + match f x with
                                        inl x' => uiterTime n' x'
                                      | _ => 0
                                      end
     end. 
 
   Lemma uiter_sound n x y:
-    loopSum n f x = Some y -> evalLe (uiterTime n x) (app uiter (enc x)) (enc y).
+    loopSum n f x = Some y -> evalLe (uiterTime n x) (app (app uiter (extT f)) (enc x)) (enc y).
   Proof.
     unfold uiter. Intern.recRem P.
     induction n in x|-*;intros Heq. now easy.
@@ -37,18 +38,43 @@ Section uiter.
     2,3:reflexivity.
     2:{
       destruct (f x) eqn:eqfx.
-      -Intern.recStepNew P. Lsimpl. rewrite eqfx. Lsimpl. eapply IHn. eauto.
+      - Intern.recStepNew P. Lsimpl. rewrite eqfx. Lsimpl. eapply IHn. eauto.
       -inv Heq. Intern.recStepNew P. Lsimpl. rewrite eqfx. Lsimpl. Lreflexivity.
     }
     destruct (f x).
     all:solverec.
   Qed.
 
+  Lemma uiter_complete x t :
+    eval (app (app uiter (extT f)) (enc x)) t -> exists n y, loopSum n f x = Some y. 
+  Proof.
+    unfold uiter. Intern.recRem P.
+    intros [k [Hk Ht]] % eval_evalIn.
+    revert x t Ht Hk. pattern k.
+    eapply complete_induction. clear k. intros k IH x t Ht Hk.
+    assert (app (extT f) (enc x) >(<= fst (fT x tt) + 0) enc (f x)). now Lsimpl. rewrite <- plus_n_O in H4.
+    destruct H4 as (? & ? & ?).
+    destruct (f x) as [x' | ] eqn:E.
+    - assert (exists i, 0 < i <= 3 + (fst (fT x tt) + 7) /\ app (app P (extT f)) (enc x) >(i) app (app P (extT f)) (enc x')).
+      eexists. split. 2:{
+      eapply pow_trans.
+      eapply pow_step_congL. eapply rho_correctPow. Lproc. Lproc. reflexivity.
+      unfold rP. Lsimpl.
+      eapply pow_trans. eapply pow_step_congL. eapply pow_step_congL. eapply pow_step_congL. exact H5.
+      all:try reflexivity.
+      eapply pow_trans with (i := 4). Lsimpl. replace (enc (@inl _ Y x')) with (lam (lam (app #1 (enc x')))) by reflexivity.
+      Lsimpl. reflexivity.
+      } cbn. lia. destruct H6 as (i & ? & ?).
+      eapply  pow_trans_lam' in H7 as (H7 & H8). 3: exact Hk. 2:Lproc.
+      eapply IH in H8 as [n H8]. 2: lia.
+      exists (S n). cbn. now rewrite E. eauto.
+    - exists 1. cbn. rewrite E. eauto.
+  Qed.
   
   Lemma uiter_total_instanceTime {Z} `{registered Z} (f':  Z -> Y) (preprocess : Z -> X) preprocessT (fuel : Z -> nat)
     `{computableTime' preprocess preprocessT} :
     (forall x, loopSum (fuel x) f (preprocess x) = Some (f' x)) ->
-    computesTime (TyArr _ _) f' (convert (λ x, !!uiter (!!(extT preprocess) x))) (fun z _ => (1 + fst (preprocessT z tt) + uiterTime (fuel z) (preprocess z),tt)).
+    computesTime (TyArr _ _) f' (convert (λ x, !!uiter !!(extT f) (!!(extT preprocess) x))) (fun z _ => (1 + fst (preprocessT z tt) + uiterTime (fuel z) (preprocess z),tt)).
   Proof.
     cbn [convert TH "-"].
     intros total.
@@ -58,7 +84,7 @@ Section uiter.
     intros ? ->.
     eexists. split. 2:reflexivity.
     eapply le_evalLe_proper. 2-3:reflexivity.
-    2:{ eapply evalLe_trans with (t := (L.app uiter (enc (preprocess z)))).
+    2:{ eapply evalLe_trans with (t := (L.app (L.app uiter (extT f)) (enc (preprocess z)))).
         -now Lsimpl.
         -eapply uiter_sound. apply total. }
     cbn.
@@ -74,7 +100,7 @@ Section uiter.
               | inr y => forall n', n <= n' -> fst (fT x tt) <= boundL + boundR n'
               end) ->
     P 0 x0 -> 
-    uiterTime n0 x0 <= n0 * (boundL + 9) + boundR n0.
+    uiterTime n0 x0 <= n0 * (boundL + 11) + boundR n0.
   Proof.
     intros H'.
     pose (n0':=n0). assert (Hleq : n0<=n0') by (cbn;lia).
@@ -95,8 +121,8 @@ Section uiter.
 
   Lemma uiterTime_bound_recRel2 (P: nat -> _ -> Prop) (iterT : X -> nat):
     (forall i x, P i x -> match f x with
-                    | inl x' => P (S i) x' /\ iterT x' + 9 + fst (fT x tt) <= iterT x
-                    | inr y => fst (fT x tt) + 9 <= iterT x
+                    | inl x' => P (S i) x' /\ iterT x' + 11 + fst (fT x tt) <= iterT x
+                    | inr y => fst (fT x tt) + 11 <= iterT x
                     end) ->
     forall n x,
       P 0 x -> 
@@ -118,8 +144,8 @@ Section uiter.
 
   Lemma uiterTime_bound_recRel (P: nat -> _ -> Prop) (iterT : nat -> X -> nat) n:
     (forall i x, P i x -> match f x with
-                    | inl x' => P (S i) x' /\ iterT (n-i-1) x' + 9 + fst (fT x tt) <= iterT (n-i) x
-                    | inr y => fst (fT x tt) + 9 <= iterT (n-i) x
+                    | inl x' => P (S i) x' /\ iterT (n-i-1) x' + 11 + fst (fT x tt) <= iterT (n-i) x
+                    | inr y => fst (fT x tt) + 11 <= iterT (n-i) x
                     end) ->
     forall x k,
       k <= n ->
@@ -152,7 +178,7 @@ Section uiter.
                 | inl x' =>  R x x'
                 | _ => True
                 end) ->
-    uiterTime k0 x0 <= k0 * (t__step + 9) + t__end.
+    uiterTime k0 x0 <= k0 * (t__step + 11) + t__end.
   Proof.
     intros H'.
     rewrite uiterTime_bound_onlyByN
@@ -174,6 +200,3 @@ Section uiter.
 End uiter.
 
 Hint Resolve uiter_proc : LProc.
-Arguments uiter _ _ _ _ _ _ _ : clear implicits.
-Arguments uiter {X Y H H0} f {fT H1}.
-
