theories/L/TM/TimeInvarianceTermination.v
@@ -1,0 +1,130 @@
+(* From Undecidability.Shared.Libs.PSL Require Import FinTypes Vectors.
+From Undecidability.L Require Import TM.TMinL.TMinL_extract.
+From Undecidability.TM Require Import Compiler_facts Compiler_spec. *)
+From Undecidability.L.Datatypes Require Import LNat Lists LProd LFinType LVector.
+From Undecidability.L Require Import Functions.FinTypeLookup Functions.EqBool.
+From Undecidability Require Import TMEncoding.
+
+Require Import Undecidability.L.TM.TMinL.TMinL_extract.
+Require Import Undecidability.L.Functions.UnboundIteration.
+From Undecidability.TM Require Import TM TM_alt TM_facts.
+Require Import Undecidability.L.Util.L_facts.
+From Undecidability.L.Datatypes Require Import LNat.
+
+Import L_Notations.
+Import HOAS_Notations.
+
+Notation PAIR := (lam (lam (lam (0 2 1)))).
+
+Section TimeInvarianceNF.
+
+Variable Σ : finType.
+
+Let reg_sig := @registered_finType Σ.
+Existing Instance reg_sig.
+
+Variable n_tps : nat.
+
+Definition s_sim : term := Eval cbn -[enc] in [L_HOAS (λ M_q0 tps, ha M_q0 (λ M q0, !!uiter M (!!PAIR q0 tps)))]. 
+
+Variable M : TM Σ n_tps.
+Variables (q q' : state M) (t t' : tapes Σ n_tps).
+
+Let reg_state := @registered_finType (state M).
+Existing Instance reg_state.
+
+Definition step_fun := (fun cfg : mconfig Σ (state M) n_tps =>
+                          if haltConf cfg then inr (ctapes cfg) else inl (TM_facts.step cfg)).
+
+Notation STEPTIME := (haltTime M + n_tps* 130+ transTime M + 185).
+
+Instance step_fun_comp : computableTime' step_fun (fun _ _ => (STEPTIME,tt)).
+Proof.
+  extract. solverec.
+Qed.
+
+Lemma TimeInvarianceNF_forward i :
+    loopSumM (M := M) (mk_mconfig q t) i = Some (mk_mconfig q' t') ->
+    evalLe (9 + i * (STEPTIME + 11) ) (s_sim ((PAIR (ext step_fun)) (enc q)) (enc t)) (enc t').
+Proof.
+  intros H.
+  assert (Hi : loopSum i step_fun (mk_mconfig q t) = Some t').
+  { clear - H.  revert H. generalize (mk_mconfig q t). intros cfg H.
+    induction i in H, cfg,t'|-*; cbn in *.
+    - congruence.
+    - unfold step_fun. destruct haltConf. inv H. reflexivity.
+      eapply IHi. eapply H.
+  }
+  eapply evalLe_trans. unfold s_sim. Lsimpl. reflexivity.
+  unshelve eapply uiter_sound in Hi. exact _. exact _. 2: eapply step_fun_comp.
+  unfold s_sim. eapply evalIn_mono. econstructor. 2:Lproc. destruct Hi as [Hi ?].
+  unfold enc at 1 in Hi. cbn in Hi. unfold enc at 1 in Hi. cbn in Hi.
+  Lsimpl. reflexivity. rewrite <- plus_n_O.
+  clear. fold (transTime M).
+  change (  uiterTime step_fun
+    (fun (_ : mconfig Σ (state M) n_tps) (_ : unit) =>
+     (haltTime M + n_tps * 130 +
+      transTime M + 185, tt)) i (mk_mconfig q t) <= i * (STEPTIME + 11)).
+  generalize STEPTIME as C. intros C. generalize (mk_mconfig q t). intros cfg. induction i in cfg |- *.
+  - cbn. lia. 
+  - cbn. destruct _. rewrite IHi. lia. lia.
+Qed.
+
+Lemma TimeInvarianceNF_backward v :
+  eval (s_sim ((PAIR (ext step_fun)) (enc q)) (enc t)) v -> exists q' t' i, loopSumM (M := M) (mk_mconfig q t) i = Some (mk_mconfig q' t').
+Proof.
+  intros H.
+  assert ((s_sim ((PAIR (ext step_fun)) (enc q)) (enc t)) >* uiter (ext step_fun) (lam (O (enc q) (enc t)))).
+  { clear H.
+    unfold s_sim. now Lsimpl. }
+  rewrite H0 in H. clear H0.
+  change (lam (O (enc q) (enc t))) with (enc (mk_mconfig q t)) in H. 
+  eapply uiter_complete in H as (n & tps' & H). clear t'. rename tps' into t'.
+  revert H. generalize (mk_mconfig q t) as cfg. intros cfg H.
+  induction n in cfg, H |- *; cbn in *.
+  - congruence.
+  - destruct step_fun eqn:E.
+    + eapply IHn in H as (q'' & t'' & i & IH). exists q'', t'', (S i). rewrite <- IH.
+      cbn.
+      unfold step_fun in E.
+      destruct haltConf; try congruence; try inv E.
+      reflexivity.
+    + inv H. unfold step_fun in E.
+      destruct haltConf eqn:EE; try congruence. inv E.
+      exists (cstate cfg), (ctapes cfg), 1. cbn. rewrite EE. now destruct cfg.
+Qed.
+
+End TimeInvarianceNF.
+
+Definition sizeTM Σ n (M : TM Σ n) := (haltTime M + n* 130+ transTime M + 185 + 11).
+
+Theorem TimeInvarianceThesis_wrt_Termination_TM_to_L :
+  forall n Σ, exists encTM : TM Σ n -> term, exists encTps : tapes Σ n -> term,
+      exists sₛᵢₘ : term, exists C1 C2 : nat, forall M : TM Σ n, forall tps,
+              (forall tps' i q',
+                  loopM (mk_mconfig (start M) tps) i = Some (mk_mconfig q' tps') ->
+                  evalLe (C1 * (S i) * sizeTM M + C2) (sₛᵢₘ (encTM M) (encTps tps)) (encTps tps')) /\
+              (forall v, eval (sₛᵢₘ (encTM M) (encTps tps)) v -> exists q' tps' i, loopM (mk_mconfig (start M) tps) i = Some (mk_mconfig q' tps')).
+Proof.
+  intros n Σ.
+  pose (reg_sig := @registered_finType Σ).
+  unshelve eexists.
+  { intros M.
+    pose (reg_state := @registered_finType (state M)).
+    unshelve refine (PAIR (extT (step_fun (M := M))) (enc (start M))). 3:eapply step_fun_comp.
+  }
+  unshelve eexists.
+  { intros tps. exact (enc tps). }
+  exists s_sim.
+  eexists 10, 10.
+  intros M tps. split.
+  - intros tps' i q' H.
+    rewrite loopSumM_loopM_iff in H.
+    eapply TimeInvarianceNF_forward in H.
+    eapply evalLe_trans_rev with (k := 9) in H as (H1 & H & _).
+    2:{ unfold s_sim. Lsimpl. } cbn -[mult].
+    unfold s_sim. 
+    eapply evalIn_mono. Lsimpl. eapply (evalIn_refl 0). Lproc.
+    fold (sizeTM M). ring_simplify. lia.
+  - intros v (q' & t' & [] & H) % TimeInvarianceNF_backward. inv H. setoid_rewrite loopSumM_loopM_iff. eauto.
+Qed.
